Bring computation monad in file

io/ILang.CompileTo.TLang.fst
@@ -6,26 +6,59 @@ open FStar.Tactics.Typeclasses
 open Hist
 open IO.Sig
 
+noeq
+type free (a:Type u#a) : Type u#(max a 1) =
+| Call : unit -> cont:(unit -> free u#a a) -> free a
+| PartialCall : (pre:pure_pre) -> cont:((squash pre) -> free u#a a) -> free a
+| Return : a -> free a
+
+//let dm_free = DMFree.dm free_cmds free_sig event free_wps
+//assume type free (a:Type)
+assume val theta : #a:Type -> free a -> hist a
+let dm_free (a:Type) (wp:hist a) =
+  tree:(free a){wp `hist_ord` theta tree} 
+
+assume val dm_free_return : (a:Type) -> (x:a) -> dm_free a (hist_return x)
+assume val dm_free_bind  : 
+  a: Type ->
+  b: Type ->
+  wp_v: Hist.hist a ->
+  wp_f: (_: a -> Prims.Tot (Hist.hist b)) ->
+  v: dm_free a wp_v ->
+  f: (x: a -> Prims.Tot (dm_free b (wp_f x))) ->
+  Tot (dm_free b (hist_bind wp_v wp_f))
+assume val dm_free_subcomp : 
+  a: Type ->
+  wp1: hist a ->
+  wp2: hist a ->
+  f: dm_free a wp1 ->
+  Pure (dm_free a wp2) (hist_ord wp2 wp1) (fun _ -> True)
+
+assume val lift_pure_dm_free :
+  a: Type ->
+  w: pure_wp a ->
+  f: (_: eqtype_as_type unit -> Prims.PURE a w) ->
+  Tot (dm_free a (wp_lift_pure_hist w))
+
+total
+reifiable
+reflectable
+effect {
+  FREEwp (a:Type) (wp : hist a) 
+  with {
+       repr       = dm_free
+     ; return     = dm_free_return
+     ; bind       = dm_free_bind 
+     ; subcomp    = dm_free_subcomp
+     }
+}
+
+sub_effect PURE ~> FREEwp = lift_pure_dm_free
+
 type resexn a = either a exn
 
-type monitorable_prop = (cmd:io_cmds) -> (io_sig.args cmd) -> (history:trace) -> Tot bool
-unfold
-let has_event_respected_pi (e:event) (check:monitorable_prop) (h:trace) : bool =
-  match e with
-  | EOpenfile arg _ -> check Openfile arg h
-  | ERead arg _ -> check Read arg h
-  | EClose arg _ -> check Close arg h
-
-let rec enforced_locally
-  (check : monitorable_prop)
-  (h l: trace) :
-  Tot bool (decreases l) =
-  match l with
-  | [] -> true
-  | e  ::  t ->
-    if has_event_respected_pi e check h then enforced_locally (check) (e::h) t
-    else false
-
+type monitorable_prop = trace -> trace -> Tot bool
+ 
 class compilable (t:Type) (pi:monitorable_prop) = {
   comp_type : Type;
   compile: t -> comp_type
@@ -39,26 +72,27 @@ instance compile_resexn (pi:monitorable_prop) (t:Type) {| d1:compilable t pi |} 
     | Inr err -> Inr err)
 }
 
-effect IIOpi (a:Type) (pi : monitorable_prop) = 
-  DM.IIO.IIOwp a (fun p h -> (forall r lt. (enforced_locally pi h lt) ==> p lt r))
-effect MIIO (a:Type) = DM.IIO.IIOwp a (Hist.trivial_hist)
+effect FREEpi (a:Type) (pi : monitorable_prop) = 
+  FREEwp a (fun p h -> (forall r lt. (pi h lt) ==> p lt r))
+effect MFREE (a:Type) = 
+  FREEwp a (fun p h -> forall lt r. p lt r)
 
-#set-options "--query_stats"
 let test_123
   (t1:Type)
   (t2:Type)
   pi
   {| d2:compilable t2 pi |} :
-  compilable (t1 -> IIOpi (resexn t2) pi) pi by (
+  (** resexn is also necessary for the PoC to work **)
+  compilable (t1 -> FREEpi (resexn t2) pi) pi by (
   (** This is needed for it to be unsound, otherwise I get an error **)
   unfold_def (`hist_return)
 ) = {
-  comp_type = t1 -> MIIO (resexn d2.comp_type);
-  compile = (fun (f:(t1 -> IIOpi (resexn t2) pi)) (x:t1) ->
-   let x : DM.IIO.dm_iio (resexn d2.comp_type) (hist_bind (fun p h -> forall r (lt: trace). enforced_locally pi h lt ==> p lt r)
-      (fun (r:resexn t2) -> hist_return (compile #_ #pi #(compile_resexn pi t2 #d2) r))) =
+  comp_type = t1 -> MFREE (resexn d2.comp_type);
+  compile = (fun (f:(t1 -> FREEpi (resexn t2) pi)) (x:t1) ->
+   let x : dm_free (resexn d2.comp_type) (hist_bind (fun p h -> forall r (lt: trace). pi h lt ==> p lt r)
+      (fun r -> hist_return (compile #_ #pi #(compile_resexn pi t2 #d2) r))) =
      reify (compile #_ #pi #(compile_resexn pi t2 #d2) (f x)) in
    assert (False);
-   DM.IIO.IIOwp?.reflect x
+   FREEwp?.reflect x
   );
 }
